<?xml version="1.0" encoding="UTF-8"?>
<!DOCTYPE rdf:RDF [
	<!ENTITY cmns-av "https://www.omg.org/spec/Commons/AnnotationVocabulary/">
	<!ENTITY cmns-cds "https://www.omg.org/spec/Commons/CodesAndCodeSets/">
	<!ENTITY cmns-cls "https://www.omg.org/spec/Commons/Classifiers/">
	<!ENTITY cmns-col "https://www.omg.org/spec/Commons/Collections/">
	<!ENTITY cmns-dsg "https://www.omg.org/spec/Commons/Designators/">
	<!ENTITY cmns-prd "https://www.omg.org/spec/Commons/ProductsAndServices/">
	<!ENTITY cmns-ra "https://www.omg.org/spec/Commons/RegistrationAuthorities/">
	<!ENTITY cmns-txt "https://www.omg.org/spec/Commons/TextDatatype/">
	<!ENTITY dct "http://purl.org/dc/terms/">
	<!ENTITY idmp-chg "https://spec.pistoiaalliance.org/idmp/ontology/META/ChangeManagement/">
	<!ENTITY idmp-dtp "https://spec.pistoiaalliance.org/idmp/ontology/ISO/ISO21090-HarmonizedDatatypes/">
	<!ENTITY idmp-eura "https://spec.pistoiaalliance.org/idmp/ontology/ISO/EuropeanJurisdiction/EuropeanRegistrationAuthorities/">
	<!ENTITY idmp-eurga "https://spec.pistoiaalliance.org/idmp/ontology/ISO/EuropeanJurisdiction/EuropeanRegulatoryAgencies/">
	<!ENTITY idmp-mprd "https://spec.pistoiaalliance.org/idmp/ontology/ISO/ISO11615-MedicinalProducts/">
	<!ENTITY idmp-spor "https://spec.pistoiaalliance.org/idmp/ontology/ISO/EuropeanJurisdiction/SubstancesProductsOrganisationsReferentials/">
	<!ENTITY idmp-sub "https://spec.pistoiaalliance.org/idmp/ontology/ISO/ISO11238-Substances/">
	<!ENTITY lcc-639-1 "https://www.omg.org/spec/LCC/Languages/ISO639-1-LanguageCodes/">
	<!ENTITY mvf "https://www.omg.org/spec/MVF/MultipleVocabularyFacility/">
	<!ENTITY owl "http://www.w3.org/2002/07/owl#">
	<!ENTITY rdf "http://www.w3.org/1999/02/22-rdf-syntax-ns#">
	<!ENTITY rdfs "http://www.w3.org/2000/01/rdf-schema#">
	<!ENTITY skos "http://www.w3.org/2004/02/skos/core#">
	<!ENTITY xsd "http://www.w3.org/2001/XMLSchema#">
]>
<rdf:RDF xml:base="https://spec.pistoiaalliance.org/idmp/ontology/ISO/EuropeanJurisdiction/SubstancesProductsOrganisationsReferentials/"
	xmlns:cmns-av="https://www.omg.org/spec/Commons/AnnotationVocabulary/"
	xmlns:cmns-cds="https://www.omg.org/spec/Commons/CodesAndCodeSets/"
	xmlns:cmns-cls="https://www.omg.org/spec/Commons/Classifiers/"
	xmlns:cmns-col="https://www.omg.org/spec/Commons/Collections/"
	xmlns:cmns-dsg="https://www.omg.org/spec/Commons/Designators/"
	xmlns:cmns-prd="https://www.omg.org/spec/Commons/ProductsAndServices/"
	xmlns:cmns-ra="https://www.omg.org/spec/Commons/RegistrationAuthorities/"
	xmlns:cmns-txt="https://www.omg.org/spec/Commons/TextDatatype/"
	xmlns:dct="http://purl.org/dc/terms/"
	xmlns:idmp-chg="https://spec.pistoiaalliance.org/idmp/ontology/META/ChangeManagement/"
	xmlns:idmp-dtp="https://spec.pistoiaalliance.org/idmp/ontology/ISO/ISO21090-HarmonizedDatatypes/"
	xmlns:idmp-eura="https://spec.pistoiaalliance.org/idmp/ontology/ISO/EuropeanJurisdiction/EuropeanRegistrationAuthorities/"
	xmlns:idmp-eurga="https://spec.pistoiaalliance.org/idmp/ontology/ISO/EuropeanJurisdiction/EuropeanRegulatoryAgencies/"
	xmlns:idmp-mprd="https://spec.pistoiaalliance.org/idmp/ontology/ISO/ISO11615-MedicinalProducts/"
	xmlns:idmp-spor="https://spec.pistoiaalliance.org/idmp/ontology/ISO/EuropeanJurisdiction/SubstancesProductsOrganisationsReferentials/"
	xmlns:idmp-sub="https://spec.pistoiaalliance.org/idmp/ontology/ISO/ISO11238-Substances/"
	xmlns:lcc-639-1="https://www.omg.org/spec/LCC/Languages/ISO639-1-LanguageCodes/"
	xmlns:mvf="https://www.omg.org/spec/MVF/MultipleVocabularyFacility/"
	xmlns:owl="http://www.w3.org/2002/07/owl#"
	xmlns:rdf="http://www.w3.org/1999/02/22-rdf-syntax-ns#"
	xmlns:rdfs="http://www.w3.org/2000/01/rdf-schema#"
	xmlns:skos="http://www.w3.org/2004/02/skos/core#"
	xmlns:xsd="http://www.w3.org/2001/XMLSchema#">
	
	<owl:Ontology rdf:about="https://spec.pistoiaalliance.org/idmp/ontology/ISO/EuropeanJurisdiction/SubstancesProductsOrganisationsReferentials/">
		<rdfs:label>Substances, Products, Organisations and Referentials (SPOR) Ontology</rdfs:label>
		<dct:abstract>The Substances, Products, Organisations and Referentials (SPOR) ontology extends the core IDMP ontologies to define additional content required to support alignment with the European Medicines Agency data management services for substances, products, organisations and referentials.</dct:abstract>
		<dct:license rdf:datatype="&xsd;anyURI">https://opensource.org/licenses/MIT</dct:license>
		<owl:imports rdf:resource="https://spec.pistoiaalliance.org/idmp/ontology/ISO/EuropeanJurisdiction/EuropeanRegistrationAuthorities/"/>
		<owl:imports rdf:resource="https://spec.pistoiaalliance.org/idmp/ontology/ISO/EuropeanJurisdiction/EuropeanRegulatoryAgencies/"/>
		<owl:imports rdf:resource="https://spec.pistoiaalliance.org/idmp/ontology/ISO/ISO11238-Substances/"/>
		<owl:imports rdf:resource="https://spec.pistoiaalliance.org/idmp/ontology/ISO/ISO11615-MedicinalProducts/"/>
		<owl:imports rdf:resource="https://spec.pistoiaalliance.org/idmp/ontology/ISO/ISO21090-HarmonizedDatatypes/"/>
		<owl:imports rdf:resource="https://spec.pistoiaalliance.org/idmp/ontology/META/ChangeManagement/"/>
		<owl:imports rdf:resource="https://www.omg.org/spec/Commons/AnnotationVocabulary/"/>
		<owl:imports rdf:resource="https://www.omg.org/spec/Commons/Classifiers/"/>
		<owl:imports rdf:resource="https://www.omg.org/spec/Commons/CodesAndCodeSets/"/>
		<owl:imports rdf:resource="https://www.omg.org/spec/Commons/Collections/"/>
		<owl:imports rdf:resource="https://www.omg.org/spec/Commons/Designators/"/>
		<owl:imports rdf:resource="https://www.omg.org/spec/Commons/ProductsAndServices/"/>
		<owl:imports rdf:resource="https://www.omg.org/spec/Commons/RegistrationAuthorities/"/>
		<owl:imports rdf:resource="https://www.omg.org/spec/Commons/TextDatatype/"/>
		<owl:imports rdf:resource="https://www.omg.org/spec/LCC/Languages/ISO639-1-LanguageCodes/"/>
		<owl:imports rdf:resource="https://www.omg.org/spec/MVF/MultipleVocabularyFacility/"/>
		<owl:versionIRI rdf:resource="https://spec.pistoiaalliance.org/idmp/ontology/ISO/20230801/EuropeanJurisdiction/SubstancesProductsOrganisationsReferentials/"/>
		<idmp-chg:hasMaturityLevel rdf:resource="&idmp-chg;Provisional"/>
		<cmns-av:copyright>Copyright (c) 2022-2023 EDM Council, Inc.</cmns-av:copyright>
		<cmns-av:copyright>Copyright (c) 2022-2023 Pistoia Alliance, Inc.</cmns-av:copyright>
	</owl:Ontology>
	
	<owl:NamedIndividual rdf:about="&idmp-eura;EuropeanMedicinesAgencyRegistrationAuthority">
		<cmns-ra:manages rdf:resource="&idmp-spor;OrganisationManagementServicesRegistry"/>
		<cmns-ra:manages rdf:resource="&idmp-spor;ProductManagementServicesRegistry"/>
		<cmns-ra:manages rdf:resource="&idmp-spor;ReferentialsManagementServicesRegistry"/>
		<cmns-ra:manages rdf:resource="&idmp-spor;SubstancesManagementServicesRegistry"/>
	</owl:NamedIndividual>
	
	<owl:NamedIndividual rdf:about="&idmp-spor;OrganisationManagementServices">
		<rdf:type rdf:resource="&cmns-ra;RegistrationService"/>
		<rdfs:label>Organisation Management Services (OMS)</rdfs:label>
		<skos:definition>services supporting a central dictionary of organisation data in multiple languages</skos:definition>
		<cmns-av:abbreviation>OMS services</cmns-av:abbreviation>
		<cmns-av:abbreviation>SPOR OMS</cmns-av:abbreviation>
		<cmns-av:directSource rdf:resource="https://spor.ema.europa.eu/omswi/"/>
		<cmns-col:isPartOf rdf:resource="&idmp-spor;SubstancesProductsOrganisationsReferentialsDataManagementServices"/>
		<cmns-prd:isProvidedBy rdf:resource="&idmp-eura;EuropeanMedicinesAgencyRegistrationAuthority"/>
	</owl:NamedIndividual>
	
	<owl:NamedIndividual rdf:about="&idmp-spor;OrganisationManagementServicesRegistry">
		<rdf:type rdf:resource="&cmns-ra;Registry"/>
		<rdfs:label>Organisation Management Services (OMS) registry</rdfs:label>
		<skos:definition>central dictionary of organisational data in multiple languages available through the Substances Products Organisations Referentials (SPOR) Organisation Management Services (RMS)</skos:definition>
		<cmns-av:abbreviation>SPOR OMS</cmns-av:abbreviation>
		<cmns-av:abbreviation>SPOR-OMS</cmns-av:abbreviation>
		<cmns-av:directSource rdf:resource="https://spor.ema.europa.eu/omswi/"/>
		<cmns-ra:isManagedBy rdf:resource="&idmp-eura;EuropeanMedicinesAgencyRegistrationAuthority"/>
	</owl:NamedIndividual>
	
	<owl:NamedIndividual rdf:about="&idmp-spor;ProductManagementServices">
		<rdf:type rdf:resource="&cmns-ra;RegistrationService"/>
		<rdfs:label>Product Management Services (PMS)</rdfs:label>
		<skos:definition>services supporting a central dictionary of product data in multiple languages</skos:definition>
		<cmns-av:abbreviation>PMS service</cmns-av:abbreviation>
		<cmns-av:abbreviation>SPOR PMS</cmns-av:abbreviation>
		<cmns-av:abbreviation>SPOR-PMS</cmns-av:abbreviation>
		<cmns-av:adaptedFrom>https://spor.ema.europa.eu/sporwi/</cmns-av:adaptedFrom>
		<cmns-col:isPartOf rdf:resource="&idmp-spor;SubstancesProductsOrganisationsReferentialsDataManagementServices"/>
		<cmns-prd:isProvidedBy rdf:resource="&idmp-eura;EuropeanMedicinesAgencyRegistrationAuthority"/>
		<cmns-ra:isManagedBy rdf:resource="&idmp-eura;EuropeanMedicinesAgencyRegistrationAuthority"/>
	</owl:NamedIndividual>
	
	<owl:NamedIndividual rdf:about="&idmp-spor;ProductManagementServicesRegistry">
		<rdf:type rdf:resource="&cmns-ra;Registry"/>
		<rdfs:label>Product Management Services (PMS) registry</rdfs:label>
		<skos:definition>central dictionary of product data in multiple languages available through the Substances Products Organisations Referentials (SPOR) Product Management Services (RMS)</skos:definition>
		<cmns-av:abbreviation>SPOR PMS</cmns-av:abbreviation>
		<cmns-av:abbreviation>SPOR-PMS</cmns-av:abbreviation>
		<cmns-av:directSource rdf:resource="https://spor.ema.europa.eu/sporwi/"/>
		<cmns-ra:isManagedBy rdf:resource="&idmp-eura;EuropeanMedicinesAgencyRegistrationAuthority"/>
	</owl:NamedIndividual>
	
	<owl:NamedIndividual rdf:about="&idmp-spor;ReferentialsManagementServices">
		<rdf:type rdf:resource="&cmns-ra;RegistrationService"/>
		<rdfs:label>Referentials Management Services (RMS)</rdfs:label>
		<skos:definition>services supporting a central dictionary of referentials data in multiple languages</skos:definition>
		<cmns-av:abbreviation>RMS service</cmns-av:abbreviation>
		<cmns-av:directSource rdf:resource="https://spor.ema.europa.eu/rmswi/"/>
		<cmns-col:isPartOf rdf:resource="&idmp-spor;SubstancesProductsOrganisationsReferentialsDataManagementServices"/>
		<cmns-prd:isProvidedBy rdf:resource="&idmp-eura;EuropeanMedicinesAgencyRegistrationAuthority"/>
		<cmns-ra:isManagedBy rdf:resource="&idmp-eura;EuropeanMedicinesAgencyRegistrationAuthority"/>
	</owl:NamedIndividual>
	
	<owl:NamedIndividual rdf:about="&idmp-spor;ReferentialsManagementServicesClassificationScheme">
		<rdf:type rdf:resource="&cmns-cls;ClassificationScheme"/>
		<rdf:type rdf:resource="&cmns-cds;CodeSet"/>
		<rdfs:label>Referentials Management Services (RMS) classification scheme</rdfs:label>
		<skos:definition>classification scheme that includes the controlled vocabularies used to classify entities included in the Substances Products Organisations Referentials (SPOR) Referentials Management Services (RMS) related services and repositories</skos:definition>
	</owl:NamedIndividual>
	
	<owl:Class rdf:about="&idmp-spor;ReferentialsManagementServicesControlledVocabulary">
		<rdfs:subClassOf rdf:resource="&idmp-dtp;ControlledVocabulary"/>
		<rdfs:subClassOf rdf:resource="&cmns-cls;ClassificationScheme"/>
		<rdfs:subClassOf rdf:resource="&cmns-cds;CodeSet"/>
		<rdfs:subClassOf>
			<owl:Restriction>
				<owl:onProperty rdf:resource="&cmns-col;isConstituentOf"/>
				<owl:hasValue rdf:resource="&idmp-spor;ReferentialsManagementServicesClassificationScheme"/>
			</owl:Restriction>
		</rdfs:subClassOf>
		<rdfs:subClassOf>
			<owl:Restriction>
				<owl:onProperty rdf:resource="&mvf;hasLanguage"/>
				<owl:hasValue rdf:resource="&lcc-639-1;English"/>
			</owl:Restriction>
		</rdfs:subClassOf>
		<rdfs:label>Referentials Management Services (RMS) controlled vocabulary</rdfs:label>
		<skos:definition>individual controlled vocabulary (list) used to classify entities included in the Substances Products Organisations Referentials (SPOR) Referentials Management Services (RMS) registry</skos:definition>
		<cmns-av:abbreviation>RMS controlled vocabulary</cmns-av:abbreviation>
		<cmns-av:synonym>RMS list</cmns-av:synonym>
	</owl:Class>
	
	<owl:Class rdf:about="&idmp-spor;ReferentialsManagementServicesControlledVocabularyTerm">
		<rdfs:subClassOf rdf:resource="&idmp-dtp;ISO21090-ConceptDescriptor"/>
		<rdfs:subClassOf rdf:resource="&cmns-cls;Classifier"/>
		<rdfs:subClassOf>
			<owl:Restriction>
				<owl:onProperty rdf:resource="&cmns-ra;isRegisteredIn"/>
				<owl:hasValue rdf:resource="&idmp-spor;ReferentialsManagementServicesRegistry"/>
			</owl:Restriction>
		</rdfs:subClassOf>
		<rdfs:subClassOf>
			<owl:Restriction>
				<owl:onProperty rdf:resource="&idmp-spor;hasSPOROtherName"/>
				<owl:onClass rdf:resource="&idmp-spor;SPOR-OtherTermName"/>
				<owl:minQualifiedCardinality rdf:datatype="&xsd;nonNegativeInteger">0</owl:minQualifiedCardinality>
			</owl:Restriction>
		</rdfs:subClassOf>
		<rdfs:subClassOf>
			<owl:Restriction>
				<owl:onProperty rdf:resource="&idmp-spor;hasSPORShortName"/>
				<owl:onClass rdf:resource="&idmp-spor;SPOR-ShortTermName"/>
				<owl:minQualifiedCardinality rdf:datatype="&xsd;nonNegativeInteger">0</owl:minQualifiedCardinality>
			</owl:Restriction>
		</rdfs:subClassOf>
		<rdfs:subClassOf>
			<owl:Restriction>
				<owl:onProperty rdf:resource="&idmp-spor;hasSPORDataClassification"/>
				<owl:onClass rdf:resource="&idmp-spor;SPOR-DataClassification"/>
				<owl:qualifiedCardinality rdf:datatype="&xsd;nonNegativeInteger">1</owl:qualifiedCardinality>
			</owl:Restriction>
		</rdfs:subClassOf>
		<rdfs:subClassOf>
			<owl:Restriction>
				<owl:onProperty rdf:resource="&idmp-spor;hasSPORDomain"/>
				<owl:onClass rdf:resource="&idmp-spor;SPOR-Domain"/>
				<owl:qualifiedCardinality rdf:datatype="&xsd;nonNegativeInteger">1</owl:qualifiedCardinality>
			</owl:Restriction>
		</rdfs:subClassOf>
		<rdfs:subClassOf>
			<owl:Restriction>
				<owl:onProperty rdf:resource="&mvf;hasStatus"/>
				<owl:onClass rdf:resource="&idmp-spor;SPOR-RecordStatus"/>
				<owl:qualifiedCardinality rdf:datatype="&xsd;nonNegativeInteger">1</owl:qualifiedCardinality>
			</owl:Restriction>
		</rdfs:subClassOf>
		<rdfs:subClassOf>
			<owl:Restriction>
				<owl:onProperty rdf:resource="&idmp-spor;hasSPORTermName"/>
				<owl:onClass rdf:resource="&idmp-spor;SPOR-TermName"/>
				<owl:qualifiedCardinality rdf:datatype="&xsd;nonNegativeInteger">1</owl:qualifiedCardinality>
			</owl:Restriction>
		</rdfs:subClassOf>
		<rdfs:subClassOf>
			<owl:Restriction>
				<owl:onProperty rdf:resource="&idmp-spor;hasSPORTermIdentifier"/>
				<owl:onDataRange rdf:resource="&xsd;string"/>
				<owl:qualifiedCardinality rdf:datatype="&xsd;nonNegativeInteger">1</owl:qualifiedCardinality>
			</owl:Restriction>
		</rdfs:subClassOf>
		<rdfs:label>Referentials Management Services (RMS) controlled vocabulary term</rdfs:label>
		<skos:definition>term in a controlled vocabulary whose values describe some substance or product from a Substances Products Organisations Referentials (SPOR) Referentials Management Services (RMS) perspective</skos:definition>
		<skos:note>SPOR Referentials Management Services (RMS) provides referentials lists and terms (such as routes of administration, dosage forms) in multiple languages. RMS supports the continuous exchange of data between information systems across the European medicines regulatory network and the pharmaceutical industry.</skos:note>
		<cmns-av:abbreviation>RMS controlled vocabulary term</cmns-av:abbreviation>
	</owl:Class>
	
	<owl:NamedIndividual rdf:about="&idmp-spor;ReferentialsManagementServicesRegistry">
		<rdf:type rdf:resource="&cmns-ra;Registry"/>
		<rdfs:label>Referentials Management Services (RMS) registry</rdfs:label>
		<skos:definition>central dictionary of referentials data in multiple languages available through the Substances Products Organisations Referentials (SPOR) Referentials Management Services (RMS)</skos:definition>
		<skos:note>SPOR Referentials Management Services (RMS) provides referentials lists and terms (such as routes of administration, dosage forms) in multiple languages. RMS supports the continuous exchange of data between information systems across the European medicines regulatory network and the pharmaceutical industry.</skos:note>
		<cmns-av:abbreviation>SPOR RMS</cmns-av:abbreviation>
		<cmns-av:abbreviation>SPOR-RMS</cmns-av:abbreviation>
		<cmns-av:directSource rdf:resource="https://spor.ema.europa.eu/rmswi/"/>
		<cmns-ra:isManagedBy rdf:resource="&idmp-eura;EuropeanMedicinesAgencyRegistrationAuthority"/>
	</owl:NamedIndividual>
	
	<owl:Class rdf:about="&idmp-spor;SPOR-DataClassification">
		<rdfs:subClassOf rdf:resource="&idmp-spor;ReferentialsManagementServicesControlledVocabularyTerm"/>
		<rdfs:label>SPOR data classification</rdfs:label>
		<skos:definition>classifier and code element that describes the nature of any data element in terms of accessibility from a Substances Products Organisations Referentials (SPOR) Referentials Management Services (RMS) perspective</skos:definition>
		<skos:example>Valid values for data classification include Confidential, Public, and Restricted.</skos:example>
		<cmns-av:directSource rdf:resource="https://spor.ema.europa.eu/v1/lists/200000004983/terms"/>
	</owl:Class>
	
	<owl:NamedIndividual rdf:about="&idmp-spor;SPOR-DataClassification-Vocabulary">
		<rdf:type rdf:resource="&idmp-spor;ReferentialsManagementServicesControlledVocabulary"/>
		<rdfs:label>SPOR data classification vocabulary</rdfs:label>
		<skos:definition>controlled vocabulary for the terms that specify the nature of any data element in terms of accessibility according to Substances Products Organisations Referentials (SPOR) Referentials Management Services (RMS)</skos:definition>
		<skos:example>Valid values for data classification include Confidential, Public, and Restricted.</skos:example>
		<cmns-dsg:hasDescription>controlled vocabulary for the terms that specify the nature of any data element in terms of accessibility according to Substances Products Organisations Referentials (SPOR) Referentials Management Services (RMS)</cmns-dsg:hasDescription>
		<mvf:hasTextualName>Data Classification</mvf:hasTextualName>
		<mvf:hasURI rdf:datatype="&xsd;anyURI">https://spor.ema.europa.eu/v1/lists/200000004983/terms</mvf:hasURI>
	</owl:NamedIndividual>
	
	<owl:Class rdf:about="&idmp-spor;SPOR-Domain">
		<rdfs:subClassOf rdf:resource="&idmp-spor;ReferentialsManagementServicesControlledVocabularyTerm"/>
		<rdfs:label>SPOR domain</rdfs:label>
		<skos:definition>classifier and code element that describes the domain in which a particular substance or product is used from a Substances Products Organisations Referentials (SPOR) Referentials Management Services (RMS) perspective</skos:definition>
		<skos:example>Valid values for record status include Human use, Veterinary use, and Human and Veterinary use.</skos:example>
		<cmns-av:directSource rdf:resource="https://spor.ema.europa.eu/v1/lists/100000000004/terms"/>
	</owl:Class>
	
	<owl:NamedIndividual rdf:about="&idmp-spor;SPOR-Domain-Vocabulary">
		<rdf:type rdf:resource="&idmp-spor;ReferentialsManagementServicesControlledVocabulary"/>
		<rdfs:label>SPOR domain vocabulary</rdfs:label>
		<skos:definition>controlled vocabulary for the terms that specify the domain in which a particular substance or product is used according to Substances Products Organisations Referentials (SPOR) Referentials Management Services (RMS)</skos:definition>
		<skos:example>Valid values for record status include Human use, Veterinary use, and Human and Veterinary use.</skos:example>
		<cmns-dsg:hasDescription>controlled vocabulary for the terms that specify the domain in which a particular substance or product is used according to Substances Products Organisations Referentials (SPOR) Referentials Management Services (RMS)</cmns-dsg:hasDescription>
		<mvf:hasTextualName>Domain</mvf:hasTextualName>
		<mvf:hasURI rdf:datatype="&xsd;anyURI">https://spor.ema.europa.eu/v1/lists/100000000004/terms</mvf:hasURI>
	</owl:NamedIndividual>
	
	<owl:Class rdf:about="&idmp-spor;SPOR-MarketingStatus">
		<rdfs:subClassOf rdf:resource="&idmp-spor;ReferentialsManagementServicesControlledVocabularyTerm"/>
		<rdfs:label>SPOR marketing status</rdfs:label>
		<skos:definition>classifier and code element that describes the current status of some substance with respect to whether or not it has been placed on the market from a Substances Products Organisations Referentials (SPOR) Referentials Management Services (RMS) perspective</skos:definition>
		<cmns-av:directSource rdf:resource="https://spor.ema.europa.eu/v1/lists/100000072052/terms"/>
	</owl:Class>
	
	<owl:NamedIndividual rdf:about="&idmp-spor;SPOR-MarketingStatus-Vocabulary">
		<rdf:type rdf:resource="&idmp-spor;ReferentialsManagementServicesControlledVocabulary"/>
		<rdfs:label>SPOR marketing status vocabulary</rdfs:label>
		<skos:definition>controlled vocabulary for the terms that describe the current status of some substance with respect to whether or not it has been placed on the market from a Substances Products Organisations Referentials (SPOR) Referentials Management Services (RMS) perspective</skos:definition>
		<cmns-dsg:hasDescription>the current status of some substance with respect to whether or not it has been placed on the market from a Substances Products Organisations Referentials (SPOR) Referentials Management Services (RMS) perspective</cmns-dsg:hasDescription>
		<mvf:hasTextualName>Marketing Status</mvf:hasTextualName>
		<mvf:hasURI rdf:datatype="&xsd;anyURI">https://spor.ema.europa.eu/v1/lists/100000072052/terms</mvf:hasURI>
	</owl:NamedIndividual>
	
	<owl:Class rdf:about="&idmp-spor;SPOR-OtherTermName">
		<rdfs:subClassOf rdf:resource="&cmns-dsg;Name"/>
		<rdfs:subClassOf>
			<owl:Restriction>
				<owl:onProperty rdf:resource="&cmns-dsg;denotes"/>
				<owl:onClass rdf:resource="&idmp-spor;ReferentialsManagementServicesControlledVocabularyTerm"/>
				<owl:qualifiedCardinality rdf:datatype="&xsd;nonNegativeInteger">1</owl:qualifiedCardinality>
			</owl:Restriction>
		</rdfs:subClassOf>
		<rdfs:label>SPOR other term name</rdfs:label>
		<skos:definition>additional (non-primary) designation for a vocabulary term in a controlled vocabulary that is part of the Substances Products Organisations Referentials (SPOR) Referentials Management Services (RMS)</skos:definition>
	</owl:Class>
	
	<owl:Class rdf:about="&idmp-spor;SPOR-RecordStatus">
		<rdfs:subClassOf rdf:resource="&idmp-spor;ReferentialsManagementServicesControlledVocabularyTerm"/>
		<rdfs:subClassOf rdf:resource="&mvf;TermStatus"/>
		<rdfs:label>SPOR record status</rdfs:label>
		<skos:definition>classifier and code element that indicates the status of the record for a vocabulary term in Substances Products Organisations Referentials (SPOR) Referentials Management Services (RMS)</skos:definition>
		<skos:example>Valid values for record status include Current, Provisional, Non-Current, and Nullified.</skos:example>
		<cmns-av:directSource rdf:resource="https://spor.ema.europa.eu/v1/lists/200000005003/terms"/>
	</owl:Class>
	
	<owl:NamedIndividual rdf:about="&idmp-spor;SPOR-RecordStatus-Vocabulary">
		<rdf:type rdf:resource="&idmp-spor;ReferentialsManagementServicesControlledVocabulary"/>
		<rdfs:label>SPOR record status vocabulary</rdfs:label>
		<skos:definition>controlled vocabulary for the terms that specify the status of a record for a vocabulary term in Substances Products Organisations Referentials (SPOR) Referentials Management Services (RMS)</skos:definition>
		<skos:example>Valid values for record status include Current, Provisional, Non-Current, and Nullified.</skos:example>
		<cmns-dsg:hasDescription>controlled vocabulary for the terms that specify the status of a record for a vocabulary term in Substances Products Organisations Referentials (SPOR) Referentials Management Services (RMS)</cmns-dsg:hasDescription>
		<mvf:hasTextualName>Record Status</mvf:hasTextualName>
		<mvf:hasURI rdf:datatype="&xsd;anyURI">https://spor.ema.europa.eu/v1/lists/200000005003/terms</mvf:hasURI>
	</owl:NamedIndividual>
	
	<owl:Class rdf:about="&idmp-spor;SPOR-RouteOfAdministration">
		<rdfs:subClassOf rdf:resource="&idmp-spor;ReferentialsManagementServicesControlledVocabularyTerm"/>
		<rdfs:subClassOf rdf:resource="&idmp-mprd;RouteOfAdministration"/>
		<rdfs:label>SPOR route of administration</rdfs:label>
		<skos:definition>classifier and code element for the path by which the pharmaceutical product is taken into or makes contact with the body in Substances Products Organisations Referentials (SPOR) Referentials Management Services (RMS)</skos:definition>
		<skos:example>Intravenous, ocular, oral, oromucosal</skos:example>
	</owl:Class>
	
	<owl:NamedIndividual rdf:about="&idmp-spor;SPOR-RouteOfAdministration-Vocabulary">
		<rdf:type rdf:resource="&idmp-spor;ReferentialsManagementServicesControlledVocabulary"/>
		<rdfs:label>SPOR route of administration vocabulary</rdfs:label>
		<skos:definition>controlled vocabulary for the path by which the pharmaceutical product is taken into or makes contact with the body in Substances Products Organisations Referentials (SPOR) Referentials Management Services (RMS)</skos:definition>
		<skos:example>Intravenous, ocular, oral, oromucosal</skos:example>
		<cmns-dsg:hasDescription>controlled vocabulary for the path by which the pharmaceutical product is taken into or makes contact with the body in Substances Products Organisations Referentials (SPOR) Referentials Management Services (RMS)</cmns-dsg:hasDescription>
		<mvf:hasTextualName>Route of Administration</mvf:hasTextualName>
	</owl:NamedIndividual>
	
	<owl:Class rdf:about="&idmp-spor;SPOR-ShelfLifeType">
		<rdfs:subClassOf rdf:resource="&idmp-spor;ReferentialsManagementServicesControlledVocabularyTerm"/>
		<rdfs:subClassOf rdf:resource="&idmp-mprd;ShelfLifeType"/>
		<rdfs:label>SPOR shelf life type</rdfs:label>
		<skos:definition>classifier and code element that describes the point in the life cycle from manufacturing to administration to a patient that a value for shelf life applies to, including potentially with respect to a specific packaging item, from a Substances Products Organisations Referentials (SPOR) Referentials Management Services (RMS) perspective</skos:definition>
		<cmns-av:directSource rdf:resource="https://spor.ema.europa.eu/v1/lists/100000073343/terms"/>
	</owl:Class>
	
	<owl:NamedIndividual rdf:about="&idmp-spor;SPOR-ShelfLifeType-Vocabulary">
		<rdf:type rdf:resource="&idmp-spor;ReferentialsManagementServicesControlledVocabulary"/>
		<rdfs:label>SPOR shelf life type vocabulary</rdfs:label>
		<skos:definition>controlled vocabulary for the terms that describe the point in the life cycle from manufacturing to administration to a patient that a value for shelf life applies to, including potentially with respect to a specific packaging item, according to Substances Products Organisations Referentials (SPOR) Referentials Management Services (RMS)</skos:definition>
		<cmns-dsg:hasDescription>controlled vocabulary for the terms that describe the point in the life cycle from manufacturing to administration to a patient that a value for shelf life applies to, including potentially with respect to a specific packaging item, according to Substances Products Organisations Referentials (SPOR) Referentials Management Services (RMS)</cmns-dsg:hasDescription>
		<mvf:hasTextualName>Shelf Life Type</mvf:hasTextualName>
		<mvf:hasURI rdf:datatype="&xsd;anyURI">https://spor.ema.europa.eu/v1/lists/100000073343/terms</mvf:hasURI>
	</owl:NamedIndividual>
	
	<owl:Class rdf:about="&idmp-spor;SPOR-ShortTermName">
		<rdfs:subClassOf rdf:resource="&cmns-dsg;Name"/>
		<rdfs:subClassOf>
			<owl:Restriction>
				<owl:onProperty rdf:resource="&cmns-dsg;denotes"/>
				<owl:onClass rdf:resource="&idmp-spor;ReferentialsManagementServicesControlledVocabularyTerm"/>
				<owl:qualifiedCardinality rdf:datatype="&xsd;nonNegativeInteger">1</owl:qualifiedCardinality>
			</owl:Restriction>
		</rdfs:subClassOf>
		<rdfs:label>SPOR short term name</rdfs:label>
		<skos:definition>shortened designation for a vocabulary term in a controlled vocabulary that is part of the Substances Products Organisations Referentials (SPOR) Referentials Management Services (RMS)</skos:definition>
	</owl:Class>
	
	<owl:Class rdf:about="&idmp-spor;SPOR-SpecialPrecautionsForStorage">
		<rdfs:subClassOf rdf:resource="&idmp-spor;ReferentialsManagementServicesControlledVocabularyTerm"/>
		<rdfs:subClassOf rdf:resource="&idmp-mprd;SpecialPrecautionsForStorage"/>
		<rdfs:label>SPOR special precautions for storage</rdfs:label>
		<skos:definition>classifier and code element that provides precise instructions for storage of a substance or product, such as the kind of container, temperature restrictions, container management, and other restrictions on the way something must be handled from a Substances Products Organisations Referentials (SPOR) Referentials Management Services (RMS) perspective</skos:definition>
		<cmns-av:directSource rdf:resource="https://spor.ema.europa.eu/v1/lists/100000073344/terms"/>
	</owl:Class>
	
	<owl:NamedIndividual rdf:about="&idmp-spor;SPOR-SpecialPrecautionsForStorage-Vocabulary">
		<rdf:type rdf:resource="&idmp-spor;ReferentialsManagementServicesControlledVocabulary"/>
		<rdfs:label>SPOR special precautions for storage vocabulary</rdfs:label>
		<skos:definition>controlled vocabulary for the terms that describe the precise instructions for storage of a substance or product, such as the kind of container, temperature restrictions, container management, and other restrictions on the way something must be handled, according to Substances Products Organisations Referentials (SPOR) Referentials Management Services (RMS)</skos:definition>
		<cmns-dsg:hasDescription>controlled vocabulary for the terms that describe the precise instructions for storage of a substance or product, such as the kind of container, temperature restrictions, container management, and other restrictions on the way something must be handled, according to Substances Products Organisations Referentials (SPOR) Referentials Management Services (RMS)</cmns-dsg:hasDescription>
		<mvf:hasTextualName>Special Precautions for Storage</mvf:hasTextualName>
		<mvf:hasURI rdf:datatype="&xsd;anyURI">https://spor.ema.europa.eu/v1/lists/100000073344/terms</mvf:hasURI>
	</owl:NamedIndividual>
	
	<owl:Class rdf:about="&idmp-spor;SPOR-TermName">
		<rdfs:subClassOf rdf:resource="&cmns-dsg;Name"/>
		<rdfs:subClassOf>
			<owl:Restriction>
				<owl:onProperty rdf:resource="&cmns-dsg;denotes"/>
				<owl:onClass rdf:resource="&idmp-spor;ReferentialsManagementServicesControlledVocabularyTerm"/>
				<owl:qualifiedCardinality rdf:datatype="&xsd;nonNegativeInteger">1</owl:qualifiedCardinality>
			</owl:Restriction>
		</rdfs:subClassOf>
		<rdfs:label>SPOR term name</rdfs:label>
		<skos:definition>designation for a vocabulary term in a controlled vocabulary that is part of the Substances Products Organisations Referentials (SPOR) Referentials Management Services (RMS)</skos:definition>
	</owl:Class>
	
	<owl:NamedIndividual rdf:about="&idmp-spor;SubstanceManagementServices">
		<rdf:type rdf:resource="&cmns-ra;RegistrationService"/>
		<rdfs:label>Substance Management Services (SMS)</rdfs:label>
		<skos:definition>services supporting a central dictionary of substance data in multiple languages</skos:definition>
		<cmns-av:abbreviation>SMS service</cmns-av:abbreviation>
		<cmns-av:directSource rdf:resource="https://spor.ema.europa.eu/smswi/"/>
		<cmns-col:isPartOf rdf:resource="&idmp-spor;SubstancesProductsOrganisationsReferentialsDataManagementServices"/>
		<cmns-prd:isProvidedBy rdf:resource="&idmp-eura;EuropeanMedicinesAgencyRegistrationAuthority"/>
		<cmns-ra:isManagedBy rdf:resource="&idmp-eura;EuropeanMedicinesAgencyRegistrationAuthority"/>
	</owl:NamedIndividual>
	
	<owl:NamedIndividual rdf:about="&idmp-spor;SubstancesManagementServicesRegistry">
		<rdf:type rdf:resource="&cmns-ra;Registry"/>
		<rdfs:label>Substances Management Services registry</rdfs:label>
		<skos:definition>central dictionary of substance data in multiple languages available through the Substances Products Organisations Referentials (SPOR) Substances Management Services (SMS)</skos:definition>
		<cmns-av:abbreviation>SPOR SMS</cmns-av:abbreviation>
		<cmns-av:abbreviation>SPOR-SMS</cmns-av:abbreviation>
		<cmns-av:directSource rdf:resource="https://spor.ema.europa.eu/smswi/"/>
		<cmns-av:explanatoryNote>SMS is currently live as an EMA internal system. Until it is onboarded in the SPOR portal, external users should use the following systems: view and search substance data in EUTCT or IRIS; submit substance change requests in the EMA Service Desk portal; Export of substance data are available at https://spor.ema.europa.eu/web-ui-data-backend/download/csv.</cmns-av:explanatoryNote>
		<cmns-ra:isManagedBy rdf:resource="&idmp-eura;EuropeanMedicinesAgencyRegistrationAuthority"/>
	</owl:NamedIndividual>
	
	<owl:NamedIndividual rdf:about="&idmp-spor;SubstancesProductsOrganisationsReferentialsDataManagementServices">
		<rdf:type rdf:resource="&cmns-ra;RegistrationService"/>
		<rdfs:label>Substances Products Organisations Referentials (SPOR) data management services</rdfs:label>
		<skos:definition>data management services for substances, products, organisations and referentials (SPOR) designed to support regulatory activities in the European Union</skos:definition>
		<cmns-av:abbreviation>SPOR</cmns-av:abbreviation>
		<cmns-av:abbreviation>SPOR data management services</cmns-av:abbreviation>
		<cmns-av:directSource rdf:resource="https://spor.ema.europa.eu/"/>
		<cmns-col:hasPart rdf:resource="&idmp-spor;OrganisationManagementServices"/>
		<cmns-col:hasPart rdf:resource="&idmp-spor;ProductManagementServices"/>
		<cmns-col:hasPart rdf:resource="&idmp-spor;ReferentialsManagementServices"/>
		<cmns-col:hasPart rdf:resource="&idmp-spor;SubstanceManagementServices"/>
		<cmns-prd:isProvidedBy rdf:resource="&idmp-eura;EuropeanMedicinesAgencyRegistrationAuthority"/>
		<cmns-ra:isManagedBy rdf:resource="&idmp-eura;EuropeanMedicinesAgencyRegistrationAuthority"/>
	</owl:NamedIndividual>
	
	<owl:ObjectProperty rdf:about="&idmp-spor;hasSPORDataClassification">
		<rdfs:subPropertyOf rdf:resource="&cmns-cls;isClassifiedBy"/>
		<rdfs:label>has SPOR data classification</rdfs:label>
		<rdfs:range rdf:resource="&idmp-spor;SPOR-DataClassification"/>
		<skos:definition>is classified by the nature of any data element in terms of accessibility</skos:definition>
	</owl:ObjectProperty>
	
	<owl:ObjectProperty rdf:about="&idmp-spor;hasSPORDomain">
		<rdfs:subPropertyOf rdf:resource="&cmns-cls;isClassifiedBy"/>
		<rdfs:label>has SPOR domain</rdfs:label>
		<rdfs:range rdf:resource="&idmp-spor;SPOR-Domain"/>
		<skos:definition>is classified by the domain in which a particular substance or product is used</skos:definition>
	</owl:ObjectProperty>
	
	<owl:ObjectProperty rdf:about="&idmp-spor;hasSPOROtherName">
		<rdfs:subPropertyOf rdf:resource="&cmns-dsg;hasName"/>
		<rdfs:label>has SPOR other name</rdfs:label>
		<rdfs:range rdf:resource="&idmp-spor;SPOR-OtherTermName"/>
		<skos:definition>provides a language-tagged string value indicating an alternate name of a given term</skos:definition>
	</owl:ObjectProperty>
	
	<owl:ObjectProperty rdf:about="&idmp-spor;hasSPORShortName">
		<rdfs:subPropertyOf rdf:resource="&cmns-dsg;hasName"/>
		<rdfs:label>has SPOR short name</rdfs:label>
		<rdfs:range rdf:resource="&idmp-spor;SPOR-ShortTermName"/>
		<skos:definition>provides a reified language-tagged string value indicating an abbreviated name of a given term</skos:definition>
	</owl:ObjectProperty>
	
	<owl:DatatypeProperty rdf:about="&idmp-spor;hasSPORTermDescription">
		<rdfs:subPropertyOf rdf:resource="&cmns-dsg;hasDescription"/>
		<rdfs:label>has SPOR term description</rdfs:label>
		<skos:definition>provides a language-tagged string value that is a textual statement describing the term</skos:definition>
	</owl:DatatypeProperty>
	
	<owl:DatatypeProperty rdf:about="&idmp-spor;hasSPORTermIdentifier">
		<rdfs:subPropertyOf rdf:resource="&cmns-txt;hasTextValue"/>
		<rdfs:label>has SPOR term identifier</rdfs:label>
		<skos:definition>provides a string valued identifier for a given SPOR term</skos:definition>
	</owl:DatatypeProperty>
	
	<owl:ObjectProperty rdf:about="&idmp-spor;hasSPORTermName">
		<rdfs:subPropertyOf rdf:resource="&cmns-dsg;hasName"/>
		<rdfs:label>has SPOR term name</rdfs:label>
		<rdfs:range rdf:resource="&idmp-spor;SPOR-TermName"/>
		<skos:definition>provides a reified language-tagged string value indicating the preferred name of a given term</skos:definition>
	</owl:ObjectProperty>

</rdf:RDF>